Direct semantics for Pallene
Small-step semantics for Pallene with progress and preservation.

pallene.v
@@ -465,3 +465,618 @@ Proof with eauto using IRTyping.
 Qed.
 
 
+
+(*
+** Direct Semantics for Pallene
+*)
+
+
+(*
+** Pallene values
+*)
+Inductive PValue : PE -> Prop :=
+| PVnil : PValue PENil
+| PVnum : forall n, PValue (PENum n)
+| PVtbl : forall a T, PValue (PETAddr a T)
+| PVfun : forall a T1 T2, PValue (PEFAddr a T1 T2)
+| PVbox : forall v, PValue v -> PValue (PECast v PTStar)
+.
+
+
+(* Canonical forms *)
+
+Lemma ValStar : forall v,
+  PValue v ->
+  MEmpty |= v : PTStar ->
+  exists v', v = PECast v' PTStar /\ PValue v'.
+Proof.
+  intros * HV HT. inversion HT; subst; inversion HV; subst; eauto.
+Qed.
+
+Lemma ValNil : forall v,
+  PValue v ->
+  MEmpty |= v : PTNil ->
+  v = PENil.
+Proof.
+  intros * HV HT. inversion HT; subst; inversion HV; subst; eauto.
+Qed.
+
+Lemma ValInt : forall v,
+  PValue v ->
+  MEmpty |= v : PTInt ->
+  exists n, v = PENum n.
+Proof.
+  intros * HV HT. inversion HT; subst; inversion HV; subst; eauto.
+Qed.
+
+Lemma ValArr : forall v T,
+  PValue v ->
+  MEmpty |= v : PTArr T ->
+  exists a, v = PETAddr a T.
+Proof.
+  intros * HV HT. inversion HT; subst; inversion HV; subst; eauto.
+Qed.
+
+Lemma ValFun : forall v T1 T2,
+  PValue v ->
+  MEmpty |= v : PTFun T1 T2 ->
+  exists a, v = PEFAddr a T1 T2.
+Proof.
+  intros * HV HT. inversion HT; subst; inversion HV; subst; eauto.
+Qed.
+
+
+(*
+** Cast a Pallene expression to a given type; gives None iff cast
+** fails.
+*)
+Fixpoint PCast (e : PE) (T : PType) : option PE :=
+  match e, T with
+  | PECast e' PTStar, PTStar => Some e		(* '*' to '*' *)
+  | PECast e' PTStar, T => PCast e' T		(* downcast from '*' *)
+  | e', PTStar => Some (PECast e' PTStar)	(* upcast to '*' *)
+  | PENil, PTNil => Some e
+  | PENum n, PTInt => Some e
+  | PETAddr a T, PTArr T' => Some (PETAddr a T')
+  | PEFAddr a T1 T2, PTFun T1' T2' => Some (PEFAddr a T1' T2')
+  | _, _ => None
+  end.
+
+(*
+** The cast of a value gives a value
+*)
+Lemma CastValue : forall e v T,
+  PValue e ->
+  PCast e T = Some v ->
+  PValue v.
+Proof.
+  intros * PV PC.
+  induction PV; destruct T; simpl in *;
+   try discriminate;
+   try (injection PC; intros; subst); auto using PValue.
+Qed.
+
+
+(*
+** A successful cast of a value to a type has that type
+*)
+Lemma CastEqType : forall e T1 T2 v,
+  PValue e ->
+  MEmpty |= e : T1 ->
+  PCast e T2 = Some v ->
+  MEmpty |= v : T2.
+Proof.
+  intros * HV HT HC.
+  remember MEmpty as Gamma eqn:HEq.
+  induction HT; inversion HV; subst;
+  destruct T2; simpl in *; try discriminate;
+  try (injection HC; intros; subst); eauto using PTyping.
+Qed.
+
+
+(*
+** A cast of a value to its own type gives the value itself
+*)
+Lemma CastToItsType : forall T v,
+  PValue v ->
+  MEmpty |= v : T ->
+  PCast v T = Some v.
+Proof.
+  intros * HV HT.
+  remember MEmpty as Gamma eqn:HEq.
+  induction HT; trivial; inversion HV; subst; trivial.
+Qed.
+
+
+(*
+** A cast to '*' never fails
+*)
+Lemma CastToStar : forall e, exists e', PCast e PTStar = Some e'.
+Proof.
+  induction e; try (eexists; simpl; eauto; fail).
+  destruct IHe.
+  destruct p;
+  simpl; eauto.
+Qed.
+
+
+Fixpoint PToIndex (n : nat) : Index := I n TgInt.
+
+
+Inductive PExpValue : Set :=
+| PEV : forall e, PValue e -> PExpValue.
+
+
+Definition PEV2Val (me : PExpValue) : PE :=
+  match me with
+  | PEV v _ => v
+  end.
+
+
+
+Inductive PMem : Set :=
+| PEmptyMem : PMem
+| PUpdateT : address -> Index -> PExpValue -> PMem -> PMem
+| PUpdateF : address -> string -> PType -> PE -> PMem -> PMem.
+
+
+Fixpoint PqueryT (a : address) (idx : nat) (m : PMem) : PE :=
+  match m with
+  | PEmptyMem => PENil
+  | PUpdateT a' idx' e m' => if Nat.eq_dec a a' then
+                           if Index_dec (PToIndex idx) idx' then (PEV2Val e)
+                           else PqueryT  a idx m'
+                         else PqueryT  a idx m'
+  | PUpdateF _ _ _ _ m' => PqueryT a idx m'
+  end.
+
+
+Fixpoint PqueryF (a : address) (m : PMem) : (string * PType * PE) :=
+  match m with
+  | PEmptyMem => (""%string, PTStar,  PENil)
+  | PUpdateT a' _ _ m' => PqueryF a m'
+  | PUpdateF a' var type body m' => if Nat.eq_dec a a' then (var, type,  body)
+                                    else PqueryF a m'
+  end.
+
+
+Fixpoint Pfreshaux (m : PMem) : address :=
+  match m with
+  | PEmptyMem => 1
+  | PUpdateT _ _ _ m' => S (Pfreshaux m')
+  | PUpdateF _ _ _ _ m' => S (Pfreshaux m')
+  end.
+
+
+Definition PfreshT (m : PMem) : (address * PMem) :=
+  let f := Pfreshaux m in
+    (f, PUpdateT f (I 0 TgNil) (PEV PENil PVnil) m).
+
+
+Definition PfreshF (m : PMem) (v : string) (t : PType) (b : PE) :
+             (address * PMem) :=
+  let f := Pfreshaux m in
+    (f, PUpdateF f v t b m).
+
+
+Reserved Notation "'[' x ':=' s ']' t" (at level 20, x constr).
+
+
+Fixpoint substitution (var : string) (y : PE)  (e : PE) : PE :=
+ match e with
+ | PENil => e
+ | PENum n => e
+ | PEPlus e1 e2 => PEPlus ([var := y] e1) ([var := y] e2)
+ | PENew _ => e
+ | PETAddr a _ => e
+ | PEFAddr a _ _ => e
+ | PEGet e1 e2 => PEGet ([var := y] e1) ([var := y] e2)
+ | PESet e1 e2 e3 => PESet ([var := y] e1) ([var := y] e2) ([var := y] e3)
+ | PEVar var' => if string_dec var var' then y else e
+ | PEFun var' T1 body T2 => if string_dec var var' then e
+                          else PEFun var' T1 ([var := y] body) T2
+ | PEApp e1 e2 => PEApp ([var := y] e1) ([var := y] e2)
+ | PECast e T => PECast ([var := y] e) T
+end
+where "'[' x ':=' s ']' t" := (substitution x s t)
+.
+
+
+(*
+** Extending an environment preserves typing
+*)
+Lemma Pinclusion_typing : forall Γ Γ' e te,
+  inclusion Γ Γ' -> Γ |= e : te -> Γ' |= e : te.
+Proof.
+  intros Γ Γ' e te Hin Hty.
+  generalize dependent Γ'.
+  induction Hty; eauto using PTyping, inclusion_update.
+Qed.
+
+
+(*
+** Particular case when extending the empty environment
+*)
+Lemma Ptyping_empty : forall Γ e te, MEmpty |= e : te -> Γ |= e : te.
+Proof.
+  eauto using Pinclusion_typing, inclusion_empty.
+Qed.
+
+
+(*
+** Substitution preserves typing
+*)
+Lemma Psubst_typing : forall e2 Γ var tv te e1,
+  (var |=> tv; Γ) |= e2 : te ->
+  MEmpty |= e1 : tv ->
+       Γ |= ([var := e1] e2) : te.
+Proof.
+  induction e2; intros Γ var tv te e1 HT2 HT1;
+  simpl; inversion HT2; subst;
+  breakStrDec;
+  eauto 6 using Pinclusion_typing, inclusion_shadow, inclusion_permute,
+    PTyping, Ptyping_empty, InNotEq.
+  - assert (te = tv). { rewrite InEq in H1. congruence. }
+      subst. eauto using Ptyping_empty.
+Qed.
+
+
+(*
+** Evaluation steps for Lir expressions
+*)
+Reserved Notation "m '/' e --> m1 '/' e1"
+(at level 40, e at level 39, m1 at level 39, e1 at level 39).
+Reserved Notation "m '/' e --> 'fail'"
+(at level 40, e at level 39).
+
+
+Inductive pstep : PMem -> PE -> PMem -> PE -> Prop :=
+| PStPlus1 : forall m e1 e2 m' e1',
+    m / e1 --> m' / e1' ->
+    m / PEPlus e1 e2 --> m' / PEPlus e1' e2
+| PStPlus2 : forall m e1 e2 m' e2',
+    PValue e1 ->
+    m / e2 --> m' / e2' ->
+    m /  PEPlus e1 e2 --> m' /  PEPlus e1 e2'
+| PStPlus : forall m n1 n2,
+    m /  PEPlus (PENum n1) (PENum n2) --> m /  PENum (n1 + n2)
+| PStNew : forall m m' free T,
+    (free, m') = PfreshT m ->
+    m / PENew T --> m' / PETAddr free T
+| PStGet1 : forall m e1 e2 m' e1',
+    m /e1 --> m' /e1' ->
+    m / PEGet e1 e2 --> m' / PEGet e1' e2
+| PStGet2 : forall m e1 e2 m' e2',
+    PValue e1 ->
+    m /e2 --> m' /e2' ->
+    m / PEGet e1 e2 --> m' / PEGet e1 e2'
+| PStGet : forall m a idx v T,
+    PCast (PqueryT a idx m) T = Some v ->
+    m / PEGet (PETAddr a T) (PENum idx) --> m / v
+| PStSet1 : forall m e1 e2 e3 m' e1',
+    m / e1 --> m' / e1' ->
+    m / PESet e1 e2 e3 --> m' / PESet e1' e2 e3
+| PStSet2 : forall m e1 e2 e3 m' e2',
+    PValue e1 ->
+    m / e2 --> m' / e2' ->
+    m / PESet e1 e2 e3 --> m' / PESet e1 e2' e3
+| PStSet3 : forall m e1 e2 e3 m' e3',
+    PValue e1 -> PValue e2 ->
+    m / e3 --> m' / e3' ->
+    m / PESet e1 e2 e3 --> m' / PESet e1 e2 e3'
+| PStSet : forall m a idx v T (Vv : PValue v),
+    PValue v ->  (* shouldn't be necessary, but otherwise it is shelved *)
+    m / PESet (PETAddr a T) (PENum idx) v -->
+            PUpdateT a (PToIndex idx) (PEV v Vv) m / PENil
+| PStFun : forall m m' v b free T1 T2,
+    (free, m') = PfreshF m v T1 b ->
+    m / PEFun v T1 b T2 --> m' / PEFAddr free T1 T2
+| PStFunapp1 : forall m e1 e2 m' e1',
+    m / e1 --> m' / e1' ->
+    m / PEApp e1 e2 --> m' / PEApp e1' e2
+| PStFunapp2 : forall m e1 e2 m' e2',
+    PValue e1 ->
+    m / e2 --> m' / e2' ->
+    m / PEApp e1 e2 --> m' / PEApp e1 e2'
+| PStFunapp : forall m a var type body v v' T1 T2,
+    PValue v ->
+    (var, type, body) = PqueryF a m ->
+    PCast v type = Some v' ->
+    m / PEApp (PEFAddr a T1 T2) v --> m / PECast ([var := v'] body) T2
+| PStCast1 : forall m e m' e' T,
+    m / e --> m' / e' ->
+    m / PECast e T --> m' / PECast e' T
+| PStCast : forall m T v v',
+    PValue v ->
+    T <> PTStar ->
+    PCast v T = Some v' ->
+    m / PECast v T --> m / v'
+
+where "m / e --> m1 / e1" := (pstep m e m1 e1).
+
+
+(*
+** Fail evaluation for Pallene expressions
+*)
+Inductive pstepF : PMem -> PE -> Prop :=
+| PStPlus1F : forall m e1 e2,
+    m / e1 --> fail ->
+    m / PEPlus e1 e2 --> fail
+| PStPlus2F : forall m e1 e2,
+    PValue e1 ->
+    m / e2 --> fail ->
+    m /  PEPlus e1 e2 --> fail
+| PStGet1F : forall m e1 e2,
+    m /e1 --> fail ->
+    m / PEGet e1 e2 --> fail
+| PStGet2F : forall m e1 e2,
+    PValue e1 ->
+    m /e2 --> fail ->
+    m / PEGet e1 e2 --> fail
+| PStGetF : forall m a idx T,
+    PCast (PqueryT a idx m) T = None ->
+    m / PEGet (PETAddr a T) (PENum idx) --> fail
+| PStSet1F : forall m e1 e2 e3,
+    m / e1 --> fail ->
+    m / PESet e1 e2 e3 --> fail
+| PStSet2F : forall m e1 e2 e3,
+    PValue e1 ->
+    m / e2 --> fail ->
+    m / PESet e1 e2 e3 --> fail
+| PStSet3F : forall m e1 e2 e3,
+    PValue e1 -> PValue e2 ->
+    m / e3 --> fail ->
+    m / PESet e1 e2 e3 --> fail
+| PStFunapp1F : forall m e1 e2,
+    m / e1 --> fail ->
+    m / PEApp e1 e2 --> fail
+| PStFunapp2F : forall m e1 e2,
+    PValue e1 ->
+    m / e2 --> fail ->
+    m / PEApp e1 e2 --> fail
+| PStFunappF : forall m a var type body v T1 T2,
+    PValue v ->
+    (var, type, body) = PqueryF a m ->
+    PCast v type = None ->
+    m / PEApp (PEFAddr a T1 T2) v --> fail
+| PStCast1F : forall m t e,
+    m / e --> fail ->
+    m / PECast e t --> fail
+| PStCastF : forall m T v,
+    PValue v ->
+    PCast v T = None ->
+    m / PECast v T --> fail
+
+ where "m / e --> 'fail'" := (pstepF m e)
+.
+
+
+Lemma ValueNormal : forall v m,
+  PValue v ->
+  ~exists e' m', m / v --> m' / e'.
+Proof.
+  intros * HV [e' [m' H]].
+  induction H; inversion HV; subst; eauto.
+Qed.
+
+Lemma ValueNormalF : forall v m,
+  PValue v ->
+  ~m / v --> fail.
+Proof.
+  intros * HV HF.
+  induction HF; inversion HV; subst; eauto.
+  specialize (CastToStar v) as [? ?].
+  congruence.
+Qed.
+
+
+
+(*
+** Ensures that all elements of tables and all "functions" in a
+** memory are well typed.
+*)
+Inductive Pmem_correct : PMem -> Prop :=
+| PMCE : Pmem_correct PEmptyMem
+| PMCT : forall a idx v m T,
+     MEmpty |= PEV2Val v : T ->
+     Pmem_correct m ->
+     Pmem_correct (PUpdateT a idx v m)
+| PMCF : forall a var type body m T,
+     var |=> type; MEmpty |= body : T ->
+     Pmem_correct m ->
+     Pmem_correct (PUpdateF a var type body m)
+.
+
+
+(*
+** All expressions stored in memory tables are values
+*)
+Lemma PMCValue : forall m a n, PValue (PqueryT a n m).
+Proof.
+  intros.
+  induction m; eauto using PValue.
+  destruct p. simpl.
+  breakIndexDec; trivial.
+Qed.
+
+
+(*
+** All expressions stored in a table of a correct memory are
+** well typed
+*)
+Lemma PMCTy : forall m a n Γ,
+    Pmem_correct m ->
+    exists T, Γ |= (PqueryT a n m) : T.
+Proof.
+  intros * H.
+  induction H; trivial.
+  - eauto using typing_empty, PTyping.
+  - simpl. breakIndexDec; subst; eauto using Ptyping_empty.
+Qed.
+
+
+(*
+** All functions stored in a correct memory have correct types.
+*)
+Lemma PMCTyF : forall m a var type body Γ,
+    (var, type,  body) = PqueryF a m ->
+    Pmem_correct m ->
+    exists T, var |=> type; Γ |= body : T.
+Proof.
+  intros * HEq HMC.
+  induction HMC; eauto.
+  - simpl in HEq. injection HEq; intros; subst.
+    eauto using PTyping.
+  - simpl in HEq. breakIndexDec; eauto.
+    injection HEq; intros; subst.
+    eauto using Pinclusion_typing, inclusion_update, inclusion_empty.
+Qed.
+
+
+(*
+** Table allocation preserves memory correctness
+*)
+Lemma Pmem_correct_freshT : forall m m' free,
+  Pmem_correct m -> (free,m') = PfreshT m -> Pmem_correct m'.
+Proof.
+  unfold freshT. intros m m' free Hmc Heq. inversion Heq.
+  eauto using Pmem_correct, PTyping.
+Qed.
+
+
+(*
+** Function allocation preserves memory correctness
+*)
+Lemma Pmem_correct_freshF : forall m m' var T1 T2 body free,
+  var |=> T1; MEmpty |= body : T2 ->
+  Pmem_correct m ->
+  (free,m') = PfreshF m var T1 body ->
+  Pmem_correct m'.
+Proof.
+  unfold PfreshF. intros * HTy Hmc Heq.
+  inversion Heq; subst.
+  eauto using Pmem_correct.
+Qed.
+
+
+(*
+** Executing an evaluation step preserves memory
+** correctness
+*)
+Lemma PmemPreservation : forall (m m' : PMem) e e' t,
+  Pmem_correct m ->
+  MEmpty |= e : t ->
+  m / e --> m' / e' ->
+  Pmem_correct m'.
+Proof.
+  intros m m' e e' t HMC HTy Hst.
+  generalize dependent m'.
+  generalize dependent e'.
+  remember MEmpty as Γ.
+  induction HTy; intros e' m' Hst; inversion Hst; subst;
+  eauto using Pmem_correct_freshT, Pmem_correct_freshF, Pmem_correct.
+Qed.
+
+
+(*
+** Preservation of types for Pallene expressions
+*)
+Lemma PexpPreservation : forall m e t m' e',
+  Pmem_correct m ->
+  MEmpty |= e : t ->
+  m / e --> m' / e' ->
+  MEmpty |= e' : t.
+Proof.
+  intros m e t m' e' Hmc HT.
+  generalize dependent m'.
+  generalize dependent e'.
+  remember MEmpty as Γ.
+  induction HT; intros e' m' Hst; inversion Hst; subst;
+  eauto using PTyping, PMCTy, PMCTyF, Psubst_typing, CastEqType.
+  - inversion HT1; subst.
+    assert (PValue (PqueryT a idx m')) by eauto using PMCValue.
+    specialize (PMCTy m' a idx MEmpty Hmc) as [T' ?].
+    eauto using CastEqType.
+  - inversion HT1; subst.
+    specialize (PMCTyF m' a var type body MEmpty H3 Hmc) as [T' ?].
+    eauto using CastEqType, CastValue, PTyCast, Psubst_typing.
+Qed.
+
+
+Ltac openCanonicValue rule :=
+  repeat match goal with
+    | [ Ht : MEmpty |= ?e : _,
+        Hv : PValue ?e |- _] =>
+          eapply rule in Ht; trivial; decompose [ex or and] Ht; clear Ht
+    end.
+
+Ltac dostep :=
+  right; only 1: (right; eauto using pstep); left;  eauto using pstepF.
+
+
+(*
+** Progress for Pallene terms
+*)
+Theorem Progress : forall m e t,
+    MEmpty |= e : t  ->
+    PValue e \/
+    (m / e --> fail \/ exists m' e', m / e --> m' / e').
+Proof.
+  intros m e t Hty.
+  remember MEmpty as Γ eqn:Heq.
+  generalize dependent m.
+  induction Hty; intros m; subst;
+
+  (* handle values *)
+    try (left; auto using PValue; fail);
+
+  (* handle variables (no variables in an empty environment) *)
+  try match goal with
+  | [ H: In MEmpty _ = Some _ |- _] => inversion H
+  end;
+
+  (* instantiate and break induction hypotheses *)
+  repeat match goal with
+    | [H: ?E = ?E -> _ |- _] =>
+      specialize (H eq_refl m) as [? | [? | [? [? ?]]]]
+  end;
+
+  (* instantiate canonic forms *)
+  openCanonicValue ValInt;
+  openCanonicValue ValArr;
+  openCanonicValue ValFun;
+  subst;
+
+  (* handle fails *)
+  try (eauto using pstepF; fail);
+
+  (* handle easy step cases *)
+  try (unshelve (right; right; subst; eauto using pstep); trivial; fail).
+
+  (* Each of the next cases needs some very specific destructs *)
+
+  - (* New *)
+    pose (PfreshT m) as P. destruct P eqn:?;
+    dostep.
+
+  - (* Get *)
+    destruct (PCast (PqueryT x0 x m) T) eqn:?; subst;
+    dostep.
+
+  - (* Fun *)
+    pose (PfreshF m var Tvar body) as P; destruct P eqn:?;
+    dostep.
+
+  - (* App *)
+    pose (PqueryF x m) as P. destruct P as [[? ?] ?] eqn:?; subst.
+    destruct (PCast e2 p) eqn:?;
+    dostep.
+
+  - (* Cast *)
+    destruct (dec_TP T2 PTStar) eqn:?; subst.
+    + (* upcast *) left. eauto using PValue.
+    + (* downcast *) destruct (PCast e T2) eqn:?;
+      dostep.
+
+Qed.
+
